Gt3/Syntax/Subst.lean
@@ -110,9 +110,9 @@ theorem Tm.Valid.bvi {k r} {a : Tm k} (h : Valid (a.erase.clamp r)) : a.bvi ≤ 
     (try constructorm* _ ∧ _) <;>
     apply_assumption <;> assumption
 
-inductive Tm.Lstn : ∀ {l r}, Tm l → Tm r → Prop
-  | refl : ∀ {l} (a : Tm l), Lstn a a
-  | lst {l r} {a : Tm l} {a' : Tm (r + 1)}
+inductive Tm.Lstn {l} (a : Tm l) : ∀ {r}, Tm r → Prop
+  | refl : Lstn a a
+  | lst {r} {a' : Tm (r + 1)}
     (h : Lstn a a') (v) : Lstn a (a'.lst v)
 
 theorem Tm.Lstn.bounds {l r} {a : Tm l} {a' : Tm r} (h : Lstn a a') : r ≤ l
@@ -146,9 +146,123 @@ theorem Tm.Lstn.clamped_valid {l r}
   rw [OTm.erase_clamp_bvi_le, h.erase_bvi] <;> convert ha.bvi
   simp
 
-inductive Tm.LstBar : ∀ {l r}, Tm l → Tm l → Tm r → Tm r → Prop
-  | refl : ∀ {l} (a b : Tm l), LstBar a b a b
-  | lst {l r} {a b : Tm l} {a' b' : Tm (r + 1)}
+theorem Tm.Lstn.fv {l r x a} (h : Lstn (l := l) (r := r) (.fv x) a) : a = .fv x := by
+  induction h <;> simp [*]
+
+theorem Tm.Lstn.univ {l r ℓ a} (h : Lstn (l := l) (r := r) (.univ ℓ) a) : a = .univ ℓ :=
+  by induction h <;> simp [*]
+
+theorem Tm.Lstn.empty {l r a} (h : Lstn (l := l) (r := r) .empty a) : a = .empty :=
+  by induction h <;> simp [*]
+
+theorem Tm.Lstn.unit {l r a} (h : Lstn (l := l) (r := r) .unit a) : a = .unit :=
+  by induction h <;> simp [*]
+
+theorem Tm.Lstn.null {l r a} (h : Lstn (l := l) (r := r) .null a) : a = .null :=
+  by induction h <;> simp [*]
+
+theorem Tm.Lstn.eqn {l r a b w} (h : Lstn (l := l) (r := r) (.eqn a b) w)
+  : ∃a' b', w = .eqn a' b' ∧ Lstn a a' ∧ Lstn b b' :=
+  by induction h with
+  | refl => exact ⟨a, b, rfl, .refl, .refl⟩
+  | lst h v I =>
+    have ⟨a', b', he, ha', hb'⟩ := I
+    exact ⟨a'.lst v, b'.lst v, by simp [he], ha'.lst v, hb'.lst v⟩
+
+theorem Tm.Lstn.pi {l r A B w} (h : Lstn (l := l) (r := r) (.pi A B) w)
+  : ∃A' B', w = .pi A' B' ∧ Lstn A A' ∧ Lstn B B' :=
+  by induction h with
+  | refl => exact ⟨A, B, rfl, .refl, .refl⟩
+  | lst h v I =>
+    have ⟨A', B', he, hA', hB'⟩ := I
+    exact ⟨A'.lst v, B'.lst v, by simp [he], hA'.lst v, hB'.lst v⟩
+
+theorem Tm.Lstn.abs {l r A b w} (h : Lstn (l := l) (r := r) (.abs A b) w)
+  : ∃A' b', w = .abs A' b' ∧ Lstn A A' ∧ Lstn b b' :=
+  by induction h with
+  | refl => exact ⟨A, b, rfl, .refl, .refl⟩
+  | lst h v I =>
+    have ⟨A', b', he, hA', hb'⟩ := I
+    exact ⟨A'.lst v, b'.lst v, by simp [he], hA'.lst v, hb'.lst v⟩
+
+theorem Tm.Lstn.app {l r f a w} (h : Lstn (l := l) (r := r) (.app f a) w)
+  : ∃f' a', w = .app f' a' ∧ Lstn f f' ∧ Lstn a a' :=
+  by induction h with
+  | refl => exact ⟨f, a, rfl, .refl, .refl⟩
+  | lst h v I =>
+    have ⟨f', a', he, hf', ha'⟩ := I
+    exact ⟨f'.lst v, a'.lst v, by simp [he], hf'.lst v, ha'.lst v⟩
+
+theorem Tm.Lstn.sigma {l r A B w} (h : Lstn (l := l) (r := r) (.sigma A B) w)
+  : ∃A' B', w = .sigma A' B' ∧ Lstn A A' ∧ Lstn B B' :=
+  by induction h with
+  | refl => exact ⟨A, B, rfl, .refl, .refl⟩
+  | lst h v I =>
+    have ⟨A', B', he, hA', hB'⟩ := I
+    exact ⟨A'.lst v, B'.lst v, by simp [he], hA'.lst v, hB'.lst v⟩
+
+theorem Tm.Lstn.pair {l r a b w} (h : Lstn (l := l) (r := r) (.pair a b) w)
+  : ∃a' b', w = .pair a' b' ∧ Lstn a a' ∧ Lstn b b' :=
+  by induction h with
+  | refl => exact ⟨a, b, rfl, .refl, .refl⟩
+  | lst h v I =>
+    have ⟨a', b', he, ha', hb'⟩ := I
+    exact ⟨a'.lst v, b'.lst v, by simp [he], ha'.lst v, hb'.lst v⟩
+
+theorem Tm.Lstn.fst {l r p w} (h : Lstn (l := l) (r := r) (.fst p) w)
+  : ∃p', w = .fst p' ∧ Lstn p p' :=
+  by induction h with
+  | refl => exact ⟨p, rfl, .refl⟩
+  | lst h v I =>
+    have ⟨p', he, hp'⟩ := I
+    exact ⟨p'.lst v, by simp [he], hp'.lst v⟩
+
+theorem Tm.Lstn.snd {l r p w} (h : Lstn (l := l) (r := r) (.snd p) w)
+  : ∃p', w = .snd p' ∧ Lstn p p' :=
+  by induction h with
+  | refl => exact ⟨p, rfl, .refl⟩
+  | lst h v I =>
+    have ⟨p', he, hp'⟩ := I
+    exact ⟨p'.lst v, by simp [he], hp'.lst v⟩
+
+theorem Tm.Lstn.dite {l r φ t e w} (h : Lstn (l := l) (r := r) (.dite φ t e) w)
+  : ∃φ' t' e', w = .dite φ' t' e' ∧ Lstn φ φ' ∧ Lstn t t' ∧ Lstn e e' :=
+  by induction h with
+  | refl => exact ⟨φ, t, e, rfl, .refl, .refl, .refl⟩
+  | lst h v I =>
+    have ⟨φ', t', e', he, hφ', ht', he'⟩ := I
+    exact ⟨φ'.lst v, t'.lst v, e'.lst v, by simp [he], hφ'.lst v, ht'.lst v, he'.lst v⟩
+
+theorem Tm.Lstn.trunc {l r A w} (h : Lstn (l := l) (r := r) (.trunc A) w)
+  : ∃A', w = .trunc A' ∧ Lstn A A' :=
+  by induction h with
+  | refl => exact ⟨A, rfl, .refl⟩
+  | lst h v I =>
+    have ⟨A', he, hA'⟩ := I
+    exact ⟨A'.lst v, by simp [he], hA'.lst v⟩
+
+theorem Tm.Lstn.choose {l r A φ w} (h : Lstn (l := l) (r := r) (.choose A φ) w)
+  : ∃A' φ', w = .choose A' φ' ∧ Lstn A A' ∧ Lstn φ φ' :=
+  by induction h with
+  | refl => exact ⟨A, φ, rfl, .refl, .refl⟩
+  | lst h v I =>
+    have ⟨A', φ', he, hA', hφ'⟩ := I
+    exact ⟨A'.lst v, φ'.lst v, by simp [he], hA'.lst v, hφ'.lst v⟩
+
+theorem Tm.Lstn.has_ty {l r A a w} (h : Lstn (l := l) (r := r) (.has_ty A a) w)
+  : ∃A' a', w = .has_ty A' a' ∧ Lstn A A' ∧ Lstn a a' :=
+  by induction h with
+  | refl => exact ⟨A, a, rfl, .refl, .refl⟩
+  | lst h v I =>
+    have ⟨A', a', he, hA', ha'⟩ := I
+    exact ⟨A'.lst v, a'.lst v, by simp [he], hA'.lst v, ha'.lst v⟩
+
+theorem Tm.Lstn.invalid {l r a} (h : Lstn (l := l) (r := r) .invalid a) : a = .invalid :=
+  by induction h <;> simp [*]
+
+inductive Tm.LstBar {l} (a b : Tm l) : ∀ {r}, Tm r → Tm r → Prop
+  | refl : LstBar a b a b
+  | lst {r} {a' b' : Tm (r + 1)}
     (h : LstBar a b a' b') (v) : LstBar a b (a'.lst v) (b'.lst v)
 
 theorem Tm.LstBar.open {l r} {a b : Tm l} {a' b' : Tm (r + 1)}
@@ -169,3 +283,194 @@ theorem Tm.LstBar.zero_left {a b a' b' : Tm 0}
 
 theorem Tm.LstBar.zero_right {a b a' b' : Tm 0}
   (h : LstBar a b a' b') : b = b' := h.rhs.zero
+
+theorem Tm.LstBar.bv {l r i a b}
+  (h : LstBar (l := l) (r := r) (.bv i) (.bv i) a b)
+  : a = b := by induction h <;> simp [*]
+
+theorem Tm.LstBar.fv {l r x a b}
+  (h : LstBar (l := l) (r := r) (.fv x) (.fv x) a b)
+  : a = .fv x ∧ b = .fv x := by simp [h.lhs.fv, h.rhs.fv]
+
+theorem Tm.LstBar.univ {l r ℓ a b}
+  (h : LstBar (l := l) (r := r) (.univ ℓ) (.univ ℓ) a b) : a = .univ ℓ ∧ b = .univ ℓ :=
+  by simp [h.lhs.univ, h.rhs.univ]
+
+theorem Tm.LstBar.empty {l r a b}
+  (h : LstBar (l := l) (r := r) .empty .empty a b) : a = .empty ∧ b = .empty :=
+  by simp [h.lhs.empty, h.rhs.empty]
+
+theorem Tm.LstBar.unit {l r a b}
+  (h : LstBar (l := l) (r := r) .unit .unit a b) : a = .unit ∧ b = .unit :=
+  by simp [h.lhs.unit, h.rhs.unit]
+
+theorem Tm.LstBar.null {l r a b}
+  (h : LstBar (l := l) (r := r) .null .null a b) : a = .null ∧ b = .null :=
+  by simp [h.lhs.null, h.rhs.null]
+
+theorem Tm.LstBar.eqn {l r al bl ar br wl wr}
+  (h : LstBar (l := l) (r := r) (.eqn al bl) (.eqn ar br) wl wr)
+  : ∃ al' bl' ar' br',
+      wl = .eqn al' bl' ∧ wr = .eqn ar' br'
+      ∧ LstBar al ar al' ar' ∧ LstBar bl br bl' br'  :=
+  by induction h with
+  | refl => exact ⟨al, bl, ar, br, rfl, rfl, .refl, .refl⟩
+  | lst h v I =>
+    have ⟨al', bl', ar', br', hl, hr, ha', hb'⟩ := I
+    exact ⟨
+      al'.lst v, bl'.lst v, ar'.lst v, br'.lst v,
+      by simp [hl], by simp [hr], ha'.lst v, hb'.lst v⟩
+
+theorem Tm.LstBar.pi {l r Al Bl Ar Br wl wr}
+  (h : LstBar (l := l) (r := r) (.pi Al Bl) (.pi Ar Br) wl wr)
+  : ∃ Al' Bl' Ar' Br',
+      wl = .pi Al' Bl' ∧ wr = .pi Ar' Br'
+      ∧ LstBar Al Ar Al' Ar' ∧ LstBar Bl Br Bl' Br'  :=
+  by induction h with
+  | refl => exact ⟨Al, Bl, Ar, Br, rfl, rfl, .refl, .refl⟩
+  | lst h v I =>
+    have ⟨Al', Bl', Ar', Br', hl, hr, hA', hB'⟩ := I
+    exact ⟨
+      Al'.lst v, Bl'.lst v, Ar'.lst v, Br'.lst v,
+      by simp [hl], by simp [hr], hA'.lst v, hB'.lst v⟩
+
+theorem Tm.LstBar.abs {l r Al bl Ar br wl wr}
+  (h : LstBar (l := l) (r := r) (.abs Al bl) (.abs Ar br) wl wr)
+  : ∃ Al' bl' Ar' br',
+      wl = .abs Al' bl' ∧ wr = .abs Ar' br'
+      ∧ LstBar Al Ar Al' Ar' ∧ LstBar bl br bl' br'  :=
+  by induction h with
+  | refl => exact ⟨Al, bl, Ar, br, rfl, rfl, .refl, .refl⟩
+  | lst h v I =>
+    have ⟨Al', bl', Ar', br', hl, hr, hA', hb'⟩ := I
+    exact ⟨
+      Al'.lst v, bl'.lst v, Ar'.lst v, br'.lst v,
+      by simp [hl], by simp [hr], hA'.lst v, hb'.lst v⟩
+
+theorem Tm.LstBar.app {l r fl al fr ar wl wr}
+  (h : LstBar (l := l) (r := r) (.app fl al) (.app fr ar) wl wr)
+  : ∃ fl' al' fr' ar',
+      wl = .app fl' al' ∧ wr = .app fr' ar'
+      ∧ LstBar fl fr fl' fr' ∧ LstBar al ar al' ar'  :=
+  by induction h with
+  | refl => exact ⟨fl, al, fr, ar, rfl, rfl, .refl, .refl⟩
+  | lst h v I =>
+    have ⟨fl', al', fr', ar', hl, hr, hf', ha'⟩ := I
+    exact ⟨
+      fl'.lst v, al'.lst v, fr'.lst v, ar'.lst v,
+      by simp [hl], by simp [hr], hf'.lst v, ha'.lst v⟩
+
+theorem Tm.LstBar.sigma {l r Al Bl Ar Br wl wr}
+  (h : LstBar (l := l) (r := r) (.sigma Al Bl) (.sigma Ar Br) wl wr)
+  : ∃ Al' Bl' Ar' Br',
+      wl = .sigma Al' Bl' ∧ wr = .sigma Ar' Br'
+      ∧ LstBar Al Ar Al' Ar' ∧ LstBar Bl Br Bl' Br'  :=
+  by induction h with
+  | refl => exact ⟨Al, Bl, Ar, Br, rfl, rfl, .refl, .refl⟩
+  | lst h v I =>
+    have ⟨Al', Bl', Ar', Br', hl, hr, hA', hB'⟩ := I
+    exact ⟨
+      Al'.lst v, Bl'.lst v, Ar'.lst v, Br'.lst v,
+      by simp [hl], by simp [hr], hA'.lst v, hB'.lst v⟩
+
+theorem Tm.LstBar.pair {l r al bl ar br wl wr}
+  (h : LstBar (l := l) (r := r) (.pair al bl) (.pair ar br) wl wr)
+  : ∃ al' bl' ar' br',
+      wl = .pair al' bl' ∧ wr = .pair ar' br'
+      ∧ LstBar al ar al' ar' ∧ LstBar bl br bl' br'  :=
+  by induction h with
+  | refl => exact ⟨al, bl, ar, br, rfl, rfl, .refl, .refl⟩
+  | lst h v I =>
+    have ⟨al', bl', ar', br', hl, hr, ha', hb'⟩ := I
+    exact ⟨
+      al'.lst v, bl'.lst v, ar'.lst v, br'.lst v,
+      by simp [hl], by simp [hr], ha'.lst v, hb'.lst v⟩
+
+theorem Tm.LstBar.fst {l r pl pr wl wr}
+  (h : LstBar (l := l) (r := r) (.fst pl) (.fst pr) wl wr)
+  : ∃ pl' pr',
+      wl = .fst pl' ∧ wr = .fst pr'
+      ∧ LstBar pl pr pl' pr'  :=
+  by induction h with
+  | refl => exact ⟨pl, pr, rfl, rfl, .refl⟩
+  | lst h v I =>
+    have ⟨pl', pr', hl, hr, hp'⟩ := I
+    exact ⟨
+      pl'.lst v, pr'.lst v,
+      by simp [hl], by simp [hr], hp'.lst v⟩
+
+theorem Tm.LstBar.snd {l r pl pr wl wr}
+  (h : LstBar (l := l) (r := r) (.snd pl) (.snd pr) wl wr)
+  : ∃ pl' pr',
+      wl = .snd pl' ∧ wr = .snd pr'
+      ∧ LstBar pl pr pl' pr'  :=
+  by induction h with
+  | refl => exact ⟨pl, pr, rfl, rfl, .refl⟩
+  | lst h v I =>
+    have ⟨pl', pr', hl, hr, hp'⟩ := I
+    exact ⟨
+      pl'.lst v, pr'.lst v,
+      by simp [hl], by simp [hr], hp'.lst v⟩
+
+theorem Tm.LstBar.dite {l r φl tl el φr tr er wl wr}
+  (h : LstBar (l := l) (r := r) (.dite φl tl el) (.dite φr tr er) wl wr)
+  : ∃ φl' tl' el' φr' tr' er',
+      wl = .dite φl' tl' el' ∧ wr = .dite φr' tr' er'
+      ∧ LstBar φl φr φl' φr' ∧ LstBar tl tr tl' tr' ∧ LstBar el er el' er'  :=
+  by induction h with
+  | refl => exact ⟨φl, tl, el, φr, tr, er, rfl, rfl, .refl, .refl, .refl⟩
+  | lst h v I =>
+    have ⟨φl', tl', el', φr', tr', er', hl, hr, hφ', ht', he'⟩ := I
+    exact ⟨
+      φl'.lst v, tl'.lst v, el'.lst v, φr'.lst v, tr'.lst v, er'.lst v,
+      by simp [hl], by simp [hr], hφ'.lst v, ht'.lst v, he'.lst v⟩
+
+theorem Tm.LstBar.trunc {l r Al Ar wl wr}
+  (h : LstBar (l := l) (r := r) (.trunc Al) (.trunc Ar) wl wr)
+  : ∃ Al' Ar',
+      wl = .trunc Al' ∧ wr = .trunc Ar'
+      ∧ LstBar Al Ar Al' Ar'  :=
+  by induction h with
+  | refl => exact ⟨Al, Ar, rfl, rfl, .refl⟩
+  | lst h v I =>
+    have ⟨Al', Ar', hl, hr, hA'⟩ := I
+    exact ⟨
+      Al'.lst v, Ar'.lst v,
+      by simp [hl], by simp [hr], hA'.lst v⟩
+
+theorem Tm.LstBar.choose {l r Al φl Ar φr wl wr}
+  (h : LstBar (l := l) (r := r) (.choose Al φl) (.choose Ar φr) wl wr)
+  : ∃ Al' φl' Ar' φr',
+      wl = .choose Al' φl' ∧ wr = .choose Ar' φr'
+      ∧ LstBar Al Ar Al' Ar' ∧ LstBar φl φr φl' φr'  :=
+  by induction h with
+  | refl => exact ⟨Al, φl, Ar, φr, rfl, rfl, .refl, .refl⟩
+  | lst h v I =>
+    have ⟨Al', φl', Ar', φr', hl, hr, hA', hφ'⟩ := I
+    exact ⟨
+      Al'.lst v, φl'.lst v, Ar'.lst v, φr'.lst v,
+      by simp [hl], by simp [hr], hA'.lst v, hφ'.lst v⟩
+
+theorem Tm.LstBar.has_ty {l r Al al Ar ar wl wr}
+  (h : LstBar (l := l) (r := r) (.has_ty Al al) (.has_ty Ar ar) wl wr)
+  : ∃ Al' al' Ar' ar',
+      wl = .has_ty Al' al' ∧ wr = .has_ty Ar' ar'
+      ∧ LstBar Al Ar Al' Ar' ∧ LstBar al ar al' ar'  :=
+  by induction h with
+  | refl => exact ⟨Al, al, Ar, ar, rfl, rfl, .refl, .refl⟩
+  | lst h v I =>
+    have ⟨Al', al', Ar', ar', hl, hr, hA', ha'⟩ := I
+    exact ⟨
+      Al'.lst v, al'.lst v, Ar'.lst v, ar'.lst v,
+      by simp [hl], by simp [hr], hA'.lst v, ha'.lst v⟩
+
+theorem Tm.LstBar.invalid {l r wl wr}
+  (h : LstBar (l := l) (r := r) .invalid .invalid wl wr) : wl = .invalid ∧ wr = .invalid :=
+  by simp [h.lhs.invalid, h.rhs.invalid]
+
+theorem Tm.LstBar.split {l r} {a b : Tm l} {a' b' : Tm r}
+  (h : LstBar a b a' b') (c : Tm l)
+  : ∃c', LstBar a c a' c' ∧ LstBar c b c' b'
+  := by induction h with
+  | refl => exact ⟨c, .refl, .refl⟩
+  | lst h v I => have ⟨c, hac, hcb⟩ := I; exact ⟨c.lst v, hac.lst v, hcb.lst v⟩
